#DONE 

related to [[session 17 Aggregate Demand, Supply, and Phillips Curve Dynamics.pdf]]

$$
W = P^eF(u, z)
$$

$$
P = (1 + \mu)W
$$

$$
\implies P = (1 + \mu)P^eF(u, z)
$$
Also, $u = 1 - \frac{N}{L}$

So, $P = (1 + \mu)P^eF(1 - \frac{Y}{L}, z)$

---

![[Pasted image 20251219100058.png]]

option B

![[Pasted image 20251219100145.png]]
option B
![[Pasted image 20251219101216.png]]



![[Pasted image 20251219100950.png]]option B

![[Pasted image 20251219101648.png]]


![[Pasted image 20251219101707.png]]

option B

![[Pasted image 20251219101911.png]]

![[Pasted image 20251219102124.png]]

![[Pasted image 20251219102230.png]]
option C

![[Pasted image 20251219102619.png]]


![[Pasted image 20251219102712.png]]


Short run Philips curve

$$
\pi = \pi^e - \alpha(u - u_n)
$$

![[Pasted image 20251219102946.png]]

![[Pasted image 20251219103027.png]]


