3 ways of measuring output:
- production 1 and 2
- income

nominal output vs real output

unemployment rate `u`

$$ u = \frac{U}{L} $$

Inflation rate: the rate at which price levels rise

$$

\pi_t = \frac{P_t - P_{t-1}}{P_{t-1}}

$$

GDP deflator is a measure of P

$$ P_t = \frac{$Y_t}{Y_t}$$

Foundation for IS-LM model

# Goods market

AD 
Z = C + I + G + X - IM
In closed economy
Z = C + I + G

`C` means consumption

$I = I_0$
$C = C(Y_D)$
where $Y_D$ is the disposable income 
$Y_D \equiv Y - T$

$C = c_0 + c_1 Y_D$
$c_1$ is the MPC
$c_0$ is the autonomous consumption

$C = c_0 + c_1 (Y - T)$

`Y` means income

From the alternative ways of measuring GDP, income is the same as output

AD

$Z = C + I + G$
$Z = c_0 + c_1 (Y - T) + I_0 + G$

In equilibrium
$Y = Z$

So,
$Y = c_0 + c_1(Y - T) + I_0 + G$

On solving for Y
$$ Y = \frac{c_0 - c_1T + I_0 - G}{1 - c_1} $$

The term $\frac{1}{1 - c_1}$ is called the multiplier


A different way,

Private Savings $S$
$$ S \equiv Y_D - C = Y - T - C $$

Government savings $S^G$

$$ S^G = T - G$$

Total Savings = $S + S^G$

In equilibrium

$$I = S + S^G$$
$$=Y - T - C + T - G = Y - C - G$$
This is the IS relation

$$Y = I + C + G$$

The paradox of savings
$$I_0 = S(Y) + S^G_0$$
so if S $\uparrow$ , Y $\downarrow$ (to restore equilibrium)

# Financial Market

Just money and bonds

Money Demand is decreasing in the interest rate

$$M^d = $YL(i)$$
![[Excalidraw/Untitled 2025-12-12 20.03.43.excalidraw]]

Central bank controls money supply $M^S$

In equilibrium $M^d = M^S$


![[Excalidraw/Untitled 2025-12-12 20.05.30.excalidraw]]

central banks dont tell $M^s$, they fix interest rate 

Expansionary monetary policy => lower interest rate. How ? By doing open market operation like buying bonds.

For a zero coupon bond, P $\uparrow$ means interest rate $\downarrow$ and vice versa

# ISLM model (basic and extended)


Investment $I$ depends on output $Y$ and interest rate $i$

$I = I(Y, i)$

$I_Y > 0$ and $I_i < 0$


So equilibrium in the Goods Market


In equilibrium
$Y = Z$

So,
$Y = C(Y - T) + I(Y, i) + G$

This is the IS relation. 












